WIP to sync with Quentin

theories/interp.v
@@ -15,9 +15,13 @@ From shack Require Import lang heap modality.
 (* the interpretation of types is simply given by
      the carrier set of the sem_typeO ofe *)
 Record interp Σ := Interp {
-    interp_car :> value → iPropO Σ;
+    interp_car :> sem_typeO Σ;
     interp_persistent v : Persistent (interp_car v)
   }.
+
+Definition interp_fun Σ (i: interp Σ) : value → iPropO Σ := interp_car Σ i.
+
+Coercion interp_fun : interp >-> Funclass.
 
 Lemma interp_car_simpl : ∀ Σ c p, @interp_car Σ (Interp _ c p) = c.
 Proof.
@@ -52,6 +56,9 @@ Section interp_cofe.
 
   Global Instance interp_car_ne n : Proper (dist n ==> (=) ==> dist n) interp_car.
   Proof. by intros A A' ? w ? <-. Qed.
+
+  Global Instance interp_car_ne2 : NonExpansive interp_car.
+  Proof. by move => n i j h. Qed.
 
   Global Instance interp_car_proper : Proper ((≡) ==> (=) ==> (≡)) interp_car.
   Proof. by intros A A' ? w ? <-. Qed.
@@ -91,7 +98,7 @@ Section proofs.
   Definition interp_nothing : interp Σ :=
     Interp (λ (_: value), False%I).
 
-   Notation ty_interpO := (lang_ty -d> listO (interpO Σ) -n> sem_typeO Σ).
+   Notation ty_interpO := (lang_ty -d> listO (interpO Σ) -n> interpO Σ).
 
    Lemma ty_interpO_ne : ∀ (rec: ty_interpO) ty, NonExpansive (rec ty).
    Proof.
@@ -101,15 +108,28 @@ Section proofs.
 
   Definition interp_fields (env: list (interp Σ)) (ftys: stringmap lang_ty) (rec: ty_interpO) :
     gmapO string (laterO (sem_typeO Σ)) :=
-    let f := λ (typ: lang_ty), Next (rec typ env) in
+    let f := λ (typ: lang_ty), Next (interp_car (rec typ env)) in
     @fmap _ _ _ (later (sem_typeO Σ)) f ftys
   .
+
+  Lemma interp_fields_env env0 env1 ftys (rec: ty_interpO):
+    (∀ ty, rec ty env0 ≡ rec ty env1) →
+    env0 ≡ env1 →
+    interp_fields env0 ftys rec ≡ interp_fields env1 ftys rec.
+  Proof.
+    rewrite /interp_fields => hrec henv.
+    induction ftys as [| s ty ftys Hs IH] using map_ind; first by constructor.
+    rewrite !fmap_insert IH.
+    do 2 f_equiv.
+    by apply hrec.
+  Qed.
 
   Lemma interp_fields_contractive ftys env: Contractive (interp_fields env ftys).
   Proof.
     rewrite /interp_fields => n i1 i2 hdist.
     apply gmap_fmap_ne_ext => k ty hin.
-    f_contractive.
+    f_contractive; simpl.
+    apply interp_car_ne2.
     by f_equiv.
   Qed.
 
@@ -133,6 +153,16 @@ Section proofs.
       (ℓ ↦ (t , interp_fields env fields rec)))%I
     ).
 
+  (* Lemma interp_class_env env0 env1 cname (rec: ty_interpO): *)
+  (*   (∀ ty, rec ty env0 ≡ rec ty env1) → *)
+  (*   env0 ≡ env1 → *)
+  (*   interp_class cname env0 rec ≡ interp_class cname env1 rec. *)
+  (* Proof. *)
+  (*   rewrite /interp_class => hrec henv v /=. *)
+  (*   do 7 f_equiv. *)
+  (*   iStartProof; iSplitR; iIntros "H". *)
+  (*   rewrite interp_fields_env. *)
+
   Definition interp_ex (cname: tag) (rec: ty_interpO): interp Σ :=
     Interp (λ (w: value), (∃ env, interp_class cname env rec w)%I).
 
@@ -148,7 +178,7 @@ Section proofs.
     Interp (λ (v: value), (interp_nonnull rec v ∨ interp_null v)%I).
 
   Definition interp_generic (env: list (interpO Σ)) (tv: nat) : interp Σ :=
-    List.nth tv env interp_nothing.
+    default interp_nothing (env !! tv).
 
   (* we use a blend of Coq/Iris recursion, the
      Coq recursion lets us handle simple structural
@@ -182,20 +212,16 @@ Section proofs.
   Proof.
     move => n x y h.
     rewrite /interp_class => v.
-    rewrite !interp_car_simpl.
+    rewrite /interp_fun !interp_car_simpl.
     do 7 f_equiv.
     rewrite mapsto_eq /mapsto_def /loc_mapsto_def.
     do 3 f_equiv.
     by apply interp_fields_ne.
   Qed.
 
-  Definition itp_rec (env: listO (interpO Σ)) (rec: ty_interpO) (ty: lang_ty)
-      : sem_typeO Σ := go env rec ty.
-
-  Local Instance itp_ne (rec: ty_interpO) (ty: lang_ty) :
-    NonExpansive (λ (env: listO (interpO Σ)), itp_rec env rec ty).
+  Local Instance go_ne (rec: ty_interpO) (ty: lang_ty) :
+    NonExpansive (λ env, go env rec ty).
   Proof.
-    rewrite /itp_rec.
     induction ty
       as [ | | | | cname targs htargs | | | A B hA hB | A B hA hB | i | cname ]
       using lang_ty_ind' => //= n x y h.
@@ -210,12 +236,12 @@ Section proofs.
       apply htargs.
       now constructor.
     - rewrite /interp_union => v.
-      rewrite !interp_car_simpl.
+      rewrite /interp_fun !interp_car_simpl.
       f_equiv.
       + revert v; by apply hA.
       + revert v; by apply hB.
     - rewrite /interp_inter => v.
-      rewrite !interp_car_simpl.
+      rewrite /interp_fun !interp_car_simpl.
       f_equiv.
       + revert v; by apply hA.
       + revert v; by apply hB.
@@ -234,7 +260,7 @@ Section proofs.
    *)
   Definition interp_type_pre (rec : ty_interpO) : ty_interpO :=
     λ (typ : lang_ty), λne (env: listO (interpO Σ)), 
-    let go_rec : lang_ty → sem_typeO Σ :=
+    let go_rec :=
     (fix go (typ: lang_ty) : interp Σ :=
       match typ with
       | IntT => interp_int
@@ -261,7 +287,7 @@ Section proofs.
   Lemma interp_class_contractive cname env: Contractive (interp_class cname env). 
   Proof.
     rewrite /interp_class => n i1 i2 hdist v.
-    rewrite !interp_car_simpl.
+    rewrite /interp_fun !interp_car_simpl.
     f_equiv ; intro l.
     f_equiv; intro t.
     f_equiv; intro fields.
@@ -274,7 +300,7 @@ Section proofs.
   Lemma interp_nonnull_contractive : Contractive interp_nonnull.
   Proof.
     rewrite /interp_nonnull => n i1 i2 hdist v.
-    rewrite !interp_car_simpl.
+    rewrite /interp_fun !interp_car_simpl.
     do 6 f_equiv.
     revert v.
     by apply interp_class_contractive.
@@ -289,8 +315,8 @@ Section proofs.
     induction ty
       as [ | | | | cname targs htargs | | | A B hA hB | A B hA hB | i | cname ]
       using lang_ty_ind' => //=.
-    - rewrite /interp_mixed => v /=.
-      rewrite !interp_car_simpl.
+    - rewrite /interp_mixed => v.
+      rewrite /interp_fun !interp_car_simpl.
       f_equiv.
       revert v; by apply interp_nonnull_contractive.
     - move => v.
@@ -309,7 +335,7 @@ Section proofs.
     - solve_proper_core ltac:(fun _ => first [done | f_contractive | f_equiv]).
     - solve_proper_core ltac:(fun _ => first [done | f_contractive | f_equiv]).
     - rewrite /interp_ex => v.
-      rewrite !interp_car_simpl.
+      rewrite /interp_fun !interp_car_simpl.
       do 2 f_equiv.
       by revert v; apply interp_class_contractive.
   Qed.
@@ -319,12 +345,231 @@ Section proofs.
      can be (mutually) recursive) *)
   Definition interp_type := fixpoint interp_type_pre.
 
+  Record interp_env := InterpEnv {
+    interp_env_car :> list (interpO Σ);
+    interp_env_as_mixed:
+      Forall (λ (e: interp Σ), ∀ v, e v -∗ interp_mixed interp_type v) interp_env_car
+  }.
+
   Lemma interp_type_unfold (env: list (interpO Σ)) (ty : lang_ty) (v : value) :
     interp_type ty env v ⊣⊢ interp_type_pre interp_type ty env v.
   Proof.
     rewrite {1}/interp_type.
     apply (fixpoint_unfold interp_type_pre ty env v).
   Qed.
+
+  Lemma interp_class_unfold env cname targs v:
+    interp_type (ClassT cname targs) env v ⊣⊢
+    interp_class cname (map (go env interp_type) targs) interp_type v.
+  Proof. by rewrite interp_type_unfold. Qed.
+
+  Lemma interp_union_unfold env A B v:
+    interp_type (UnionT A B) env v ⊣⊢
+    interp_union (interp_type A env) (interp_type B env) v.
+  Proof.
+    rewrite interp_type_unfold /=.
+    iSplit; iIntros "[H | H]".
+    - iLeft; by rewrite interp_type_unfold.
+    - iRight; by rewrite interp_type_unfold.
+    - iLeft; by rewrite interp_type_unfold.
+    - iRight; by rewrite interp_type_unfold.
+  Qed.
+
+  Lemma interp_inter_unfold env A B v:
+    interp_type (InterT A B) env v ⊣⊢
+    interp_inter (interp_type A env) (interp_type B env) v.
+  Proof.
+    rewrite interp_type_unfold /=.
+    iSplit; iIntros "[HL HR]".
+    - rewrite !interp_type_unfold; by iSplit.
+    - rewrite !interp_type_unfold; by iSplit.
+  Qed.
+
+  Lemma interp_type_go env ty :
+    go env interp_type ty ≡ interp_type ty env.
+  Proof.
+    move => v.
+    rewrite interp_type_unfold /=.
+    by elim: ty.
+  Qed.
+
+  Lemma interp_type_env_ext env0 env1 ty v:
+    (env0 ≡ env1)%I -∗
+    interp_type ty env0 v  ∗-∗ interp_type ty env1 v.
+  Proof.
+    iIntros "H".
+    iRewrite "H".
+    iSplit; by iIntros "H".
+  Qed.
+
+  Lemma interp_type_map_go fty env targs v:
+    interp_type fty (map (go env interp_type) targs) v ⊣⊢
+    interp_type fty (map (λ ty : lang_ty, interp_type ty env) targs) v.
+  Proof.
+    iApply interp_type_env_ext.
+    iApply list_equivI.
+    iIntros (n).
+    rewrite !list_lookup_fmap.
+    destruct (decide (n < length targs)) as [heq | hne].
+    - apply lookup_lt_is_Some_2 in heq as [ty ->].
+      rewrite option_equivI; simpl.
+      by rewrite interp_type_go.
+    - rewrite !lookup_ge_None_2 /=; last by lia.
+      done.
+  Qed.
+
+  (*
+  (* MOVE TO HELPER FILE / STDPP *)
+  Section fmap.
+    Context {A B : Type} (f : A → B).
+    Implicit Types l : list A.
+    Lemma list_fmap_equiv_ext_in `{!Equiv B} (g : A → B) l :
+      (∀ x, x ∈ l → f x ≡ g x) → f <$> l ≡ g <$> l.
+    Proof.
+      induction l as [ | hd tl hi] => h //=; first by constructor.
+      constructor.
+      - apply h; by constructor.
+      - apply hi => x hx; apply h; by constructor.
+    Qed.
+  End fmap.
+
+  Lemma go_subst ty : ∀ env targs v,
+    go (map (λ ty0 : lang_ty, interp_type ty0 env) targs) interp_type ty v ⊣⊢
+    go env interp_type (subst targs ty) v.
+  Admitted.
+  (*
+  Proof.
+    induction ty
+      as [ | | | | cname args hargs | | | A B hA hB | A B hA hB | i | cname ]
+      using lang_ty_ind' => env targs //=.
+    - rewrite map_map.
+      assert (hmap:
+        (map (go (map (λ ty0 : lang_ty, interp_type ty0 env) targs) interp_type) args) ≡
+        (map (λ x : lang_ty, go env interp_type (subst targs x)) args)).
+      { apply list_fmap_equiv_ext_in => x hx.
+        rewrite Forall_forall in hargs.
+        by rewrite hargs; last done.
+      }
+      rewrite hmap.
+
+      { rewrite map_map.
+        apply list_equivI.
+        apply map_ext_in  => a /elem_of_list_In ha.
+      rewrite Forall_forall in hargs.
+      apply hargs.
+    - by rewrite hA hB.
+    - by rewrite hA hB.
+    - rewrite /interp_generic. 
+      rewrite list_lookup_fmap.
+      destruct (decide (i < length targs)) as [ hlt | hge].
+      + apply lookup_lt_is_Some_2 in hlt as [a ->] => /=.
+        symmetry.
+        rewrite interp_type_go.
+lookup_lt_is_Some_2:
+  ∀ (A : Type) (l : list A) (i : nat), i < length l → is_Some (l !! i)
+      Search lookup "map".
+
+      replace interp_nothing with (interp_type NothingT env); last first.
+      { rewrite interp_type_unfold .
+      rewrite map_nth.
+
+
+  Qed.
+
+   *)
+  (* Lemma *) 
+  (*       assert (hmap: *)
+  (*         (map (go (map (λ ty : lang_ty, interp_type ty env) fargs) interp_type) targs) = *)
+  (*         (map (λ x : lang_ty, go env interp_type (subst fargs x)) targs) *)
+  (*       ). *)
+
+  Lemma interp_type_subst fty fargs env w:
+    interp_type fty (map (λ ty : lang_ty, interp_type ty env) fargs) w -∗
+    interp_type (subst fargs fty) env w.
+  Proof.
+    rewrite !interp_type_unfold.
+    revert w.
+    induction fty
+      as [ | | | | cname targs htargs | | | A B hA hB | A B hA hB | i | cname ]
+      using lang_ty_ind' => // w.
+      - rewrite -!interp_type_unfold !interp_class_unfold.
+        fold subst.
+        rewrite map_map.
+        iIntros "H".
+        iDestruct "H" as (l t fields) "[%H Hl]".
+        destruct H as [-> [hin hfs]].
+        iExists l, t, fields; iSplitR; first done.
+        assert (hmap:
+          (map (go (map (λ ty : lang_ty, interp_type ty env) fargs) interp_type) targs) =
+          (map (λ x : lang_ty, go env interp_type (subst fargs x)) targs)
+        ).
+        admit.
+        rewrite hmap.
+        done.
+        admit.
+        iRewrite "hmap".
+
+
+
+        admit.
+        iIntros "H".
+        rewrite map_map.
+        iRewrite "hmap".
+        iDestruct "H" as (l t fields) "[%H Hl]".
+        destruct H as [-> [hin hfs]].
+        iExists l, t, fields; iSplitR; first done.
+        assert (hmap:
+              (map (go (map (λ ty : lang_ty, interp_type ty env) fargs) interp_type) targs)
+              =
+              (map (λ x : lang_ty, go env interp_type (subst fargs x)) targs)
+              ).
+              clear cname l t fields hin hfs.
+              apply map_ext_in => ty hin.
+
+
+
+    - rewrite -interp_type_unfold interp_union_unfold.
+      iIntros "[H | H]".
+      + iLeft.
+        iApply hA.
+        by rewrite -interp_type_unfold.
+      + iRight.
+        iApply hB.
+        by rewrite -interp_type_unfold.
+    - rewrite -interp_type_unfold interp_inter_unfold.
+      iIntros "[HL HR]".
+      iSplit.
+      + iApply hA.
+        by rewrite -interp_type_unfold.
+      + iApply hB.
+        by rewrite -interp_type_unfold.
+    - iAssert (∀ i j, ⌜i ≤ j⌝ -∗
+        nth i (map (λ ty : lang_ty, interp_type ty env) fargs) interp_nothing w -∗
+        (fix go (typ : lang_ty) : interp Σ :=
+        match typ with
+        | IntT => interp_int
+        | BoolT => interp_bool
+        | NothingT => interp_nothing
+        | MixedT => interp_mixed interp_type
+        | ClassT t targs => interp_class t (map go targs) interp_type
+        | NullT => interp_null
+        | NonNullT => interp_nonnull interp_type
+        | UnionT A B => interp_union (go A) (go B)
+        | InterT A B => interp_inter (go A) (go B)
+        | GenT n => nth n env interp_nothing
+        | ExT cname => interp_ex cname interp_type
+        end) (nth i fargs (GenT j)) w
+        )%I as "Hgen".
+      { iIntros (x y) "%hxy"; simpl; rewrite /interp_generic; iIntros "H". 
+        iInduction fargs as [ | hd tl hi] "IH" forall (x y hxy) => //=; first by destruct x.
+        destruct x as [ | x]; first by rewrite interp_type_unfold.
+        iApply "IH"; last done.
+        iPureIntro; by lia.
+      }
+      iApply "Hgen".
+      by iPureIntro.
+  Qed.
+   *)
 
   (* #hyp *)
   Global Instance interp_type_persistent :
@@ -357,20 +602,16 @@ Section proofs.
     by iFrame.
   Qed.
 
-  Definition env_as_mixed (env : list (interpO Σ)) :=
-    Forall (λ (e: interp Σ), ∀ v, e v -∗ interp_mixed interp_type v) env.
-
   (* A <: B → ΦA ⊂ ΦB *)
   Theorem subtype_is_inclusion_aux:
     ∀ (A B: lang_ty), A <: B →
-    ∀ env v,
-    env_as_mixed env →
+    ∀ (env: interp_env) v,
     interp_type_pre interp_type A env v -∗
     interp_type_pre interp_type B env v.
   Proof.
     induction 1 as [A | A B hext | | | | A | A B| A B | A B C h0 hi0 h1 hi1
         | A B | A B | A B C h0 hi0 h1 hi1 | A | A B C h0 hi0 h1 hi1 | cname targs ];
-    move => env v henv /=.
+    move => env v /=.
     - rewrite /interp_mixed.
       elim: A v => //=.
       + move => v; iIntros "h"; by repeat iLeft.
@@ -394,14 +635,15 @@ Section proofs.
       + move => tvar v.
         rewrite /interp_generic.
         iIntros "hv".
-        rewrite /env_as_mixed Forall_forall in henv.
+        destruct env as [env henv] => /=.
+        rewrite Forall_forall in henv.
         destruct (decide (tvar < length env)) as [hlt | hge].
         * iApply henv; last done.
-          apply elem_of_list_In.
-          apply nth_In.
-          by apply hlt.
-        * rewrite nth_overflow; first done.
-          by apply not_lt.
+          apply lookup_lt_is_Some_2 in hlt as [ t ht ].
+          rewrite ht /=.
+          by apply elem_of_list_lookup_2 in ht.
+        * rewrite lookup_ge_None_2 /=; last by apply not_lt.
+          done.
       + move => cname v;
         rewrite /interp_ex.
         iIntros "hv".
@@ -440,10 +682,10 @@ Section proofs.
 
   Theorem subtype_is_inclusion:
     ∀ A B, A <: B →
-    ∀ env, env_as_mixed env →
+    ∀ (env: interp_env),
     ∀ v, interp_type A env v -∗ interp_type B env v.
   Proof.
-    move => A B hAB env henv v.
+    move => A B hAB env v.
     rewrite !interp_type_unfold.
     by iApply subtype_is_inclusion_aux.
   Qed.
@@ -453,14 +695,13 @@ Section proofs.
     (∀ v ty, ⌜lty !! v = Some ty⌝ -∗
     ∃ val, ⌜le !! v = Some val⌝ ∗ interp_type ty env val)%I.
 
-  Lemma interp_local_tys_is_inclusion (env: list (interpO Σ))  lty rty le:
-    env_as_mixed env →
+  Lemma interp_local_tys_is_inclusion (env: interp_env)  lty rty le:
     Forall (λ (i: interp Σ), ∀ v, Persistent (i v)) env →
     lty <:< rty →
     interp_local_tys env lty le -∗
     interp_local_tys env rty le.
   Proof.
-    move => henv hpers hsub; iIntros "Hle" (v ty) "%Hv".
+    move => hpers hsub; iIntros "Hle" (v ty) "%Hv".
     apply hsub in Hv as (B & hB & hsubB).
     iDestruct ("Hle" $! v B hB) as (val) "[%Hv' #H]".
     iExists val; iSplitR; first done.
